\section{Computing Non-relational collecting}
\label{sec:computingnonrel}

In this section we argue that the same method we used in
section~\ref{sec:computingint} can be appied to the non-relational
collecting abstraction in order to compute it in finite time without
widening and narrowing operators, and therefore solve the following
problem

\begin{problem}[Termination of non-relational
  analysis]\label{p:nonrel}
  Given \(\com\in\imp, \eta \in \bCnr\), decide
  \(\semnr{\com}\eta =^? \top\)
\end{problem}

To do so we prove the same property of Lemma~\ref{le:inc}, this time
for the non-relational collecting semantics of
Definition~\ref{def:nonrel}, and therefore derive the decidability of
Problem~\ref{p:nonrel}.

\begin{lemma}
  \label{le:incnr}
  Let \(\com\in \imp\). % and \(\var[y] \in \Var\)
    
  \noindent
  For all \(\eta \in \bCnr\) and \(\var[y] \in \Var\), if
  \(\max(\semnr{\com} \eta \var[y]) \neq \infty\) and
  \(\max(\semnr{\com}\eta \var[y]) > \bound{\com}\) then there exist a
  variable \(\var[z] \in \Var\) and an integer \(h \in \mathbb{Z}\)
  such that \(|h| \leq \bound{\com}\) and the following two properties
  hold:
  \begin{enumerate}[label=(\roman*)]
  \item \(\max(\semnr{\com}\eta \var[y]) = \max(\eta \var[z]) + h\); \label{point1nr}
  \item  for all \(\eta' \in \bCnr\), if \(\eta' \nrsupseteq \eta\)
    % and \(\semnr{\com}\eta' \neq \top\)
    then
    \(\max(\semnr{\com}\eta' \var[y]) \geq \max(\eta' \var[z]) + h\). \label{point2nr}
  \end{enumerate}
\end{lemma}

\begin{proof}
  The proof is by structural induction on the command \(\com\in \imp\).
  %
  We preliminarly observe that we can safely assume
  \(\eta \neq \bot\).
  % In fact, if \(\eta = \top\) then \(\semnr{\com} \eta = \top\), so that the
  % hypothesis \(\semnr{\com} \eta \neq \top\) would not
  % be satisfied.
  In fact, if \(\eta = \bot\) then \(\semnr{\com} \bot = \bot\) and
  thus \(\max(\semnr{\com} \eta \var[y]) = 0 \leq \bound{\com}\),
  against the hypothesis
  \(\max(\semnr{\com}\eta \var[y]) > \bound{\com}\). Moreover, when
  quantifying over \(\eta'\) such that \(\eta' \dot{\supseteq} \eta\) in
  \ref{point1nr}, if \(\max(\semnr{\com}\eta' \var[y]) = \infty\)
  holds, then
  \(\max(\semnr{\com}\eta' \var[y]) \geq \max(\eta' \var[z]) + h\)
  trivially holds, hence we will sometimes silently omit to consider
  this case.
  
  \medskip
  
  \noindent
  \textbf{Case} (\(\var \in S\))\\
  % 
  Take \(\eta \in \bCnr\) and assume
  \(\infty\neq\max(\semnr{\var \in S}\eta \var[y]) > \bound{\var \in
    S}\).
  %
  Clearly \(\semnr{\var \in S}\eta \neq \bot\), otherwise
  \(\max(\semnr{\var \in S}\eta \var[y]) =0 \leq \bound{\var \in S}\)
  which is against the hypothesis that
  \(\max(\semnr{\var \in S}\eta \var[y]) > \bound{\var \in S}\)
  
  We distinguish two cases:
  \begin{itemize}
    
  \item If \(\var[y] \neq \var\), then for all \(\eta' \in \bCnr\)
    such that \(\eta \nrsubseteq \eta'\) it holds
    \(\bot \neq \semnr{\var \in S}\eta' = \eta'[\var \mapsto \eta\var
      \cap S]\) and thus
    \[
    \max(\semnr{\var \in S}\eta' \var[y]) = \max(\eta' \var[y]) = \max(\eta' \var[y]) + 0
    \]
    hence the thesis follows with \(\var[z]=\var[y]\) and \(h = 0\).

  \item If \(\var[y] = \var[x]\) then  \(\eta\var \subseteq \n\) and
    \begin{equation*}
      \max(\semnr{\var \in S}\eta \var[y]) = \max (\eta\var \cap S)
    \end{equation*}
    Note that it cannot be \(\max(S)\in \nat\). Otherwise, by
    Definition~\ref{de:bound},
    \(\max (\eta\var \cap S) \leq \max(S)= \bound{\var \in S}\),
    violating the assumption
    \(\max(\semnr{\var \in S}\eta \var[y]) > \bound{\var \in S}\).
    Hence, \(\max(S) = \infty\) must hold and therefore
    \(\max (\eta\var \cap S) = \max(\eta\var)= \max(\eta\var)+0\).
    It is immediate to check that the same holds for all
    \(\eta' \nrsupseteq \eta\), i.e.,
    \begin{equation*}
      \max (\eta'\var \cap S) = \max(\eta'\var)=
      \max(\eta'\var)+0
    \end{equation*}
    and thus the thesis follows with \(\var[z]=\var[y]=\var[x]\) and
    \(h=0\).
  \end{itemize}  
  
  % \medskip
  
  % \noindent
  % \textbf{Case} (\(\tru\))
  % A consequence of the fact that \(\tru \equiv x\in \nat\). 

  % \medskip
  
  % \noindent
  % \textbf{Case} (\(\ff\))
  % A consequence of the fact that \(\ff \equiv x\in \varnothing\). 
  %
  %  Since \(\semnr{\ff}\eta = \bot\) and thus
  %  \begin{center}
  %    \(\max(\semnr{\ff}\eta \var[y]) = \max(\bot \var[y]) =0 \leq \bound{\ff}\).
  %  \end{center}
  %  the thesis vacuosly holds


  % ----------------------------------------------
  
  \medskip
  
  \noindent
  \textbf{Case} (\(\var := k\))
  % 
  Take \(\eta \in \bCnr\) and assume
  \(\max(\semnr{\var := k}\eta \var[y]) > \bound{\var := k} = k\).

  Observe that it cannot be \(\var = \var[y]\). In fact, since
  \(\semnr{\var := k}\eta = \eta[\var \mapsto \{k\}]\), we would have
  \(\semnr{\var := k}\eta \var[y] = \{k\}\) and thus
  \begin{center}
    \(\max(\semnr{\var := k}\eta \var[y]) = k  = \bound{\var := k}\).
  \end{center}
  violating the assumption.
  %
  Therefore, it must be \(\var[y] \neq \var\). Now, for all
  \(\eta' \nrsupseteq \eta\), we have
  \(\semnr{\var := k}\eta' \var[y] = \eta' \var[y]\) and thus
  \begin{center}
    \(\max(\semnr{\var := k}\eta' \var[y]) = \max(\eta' \var[y]) =
    \max(\eta' \var[y]) + 0\),
  \end{center}
  hence the thesis holds with \(h =0 \leq \bound{\var :=k}\) and \(\var[z] = \var[y]\).
  

  % ----------------------------------------------
  
  \medskip
  
  \noindent
  \textbf{Case} (\(\var := \var[w] + k\))
  % 
  Take \(\eta \in \bCnr\) and assume
  \(\max(\semnr{\var := \var[w] + k}\eta \var[y]) > \bound{\var := \var[w] + k} = k\).
  %
  Recall that
  \(\semnr{\var := \var[w] + k}\eta = \eta[\var \mapsto \eta \var[w] + k]\).
  
  We distinguish two cases:
  \begin{itemize}
    
  \item If \(\var[y] \neq \var\), then for all \(\eta' \nrsupseteq \eta\), we have
    \(\semnr{\var := \var[w] + k}\eta' \var[y] = \eta' \var[y]\) and thus
    \begin{center}
      \(\max(\semnr{\var := \var[w] + k}\eta' \var[y]) = \max(\eta' \var[y])\).
    \end{center}
    hence the thesis follows with
    \(h =0 \leq \bound{\var := \var[w] + k}\) and \(\var[z] = \var[y]\).
    
  \item 
    If \(\var = \var[y]\) then  for all \(\eta' \nrsupseteq \eta\), we have
    \(\semnr{\var := \var[w] + k}\eta' \var[y] = \eta' \var[w] +
    k\) and thus
    \begin{center}
      \(\max(\semnr{\var := \var[w] + k}\eta' \var[y]) = \max(\eta' \var[w]) +
      k\).
    \end{center}
    
    Hence, the thesis follows with \(h = k \leq \bound{\var := \var[w] + k}\)
    and \(\var[z] = \var[w]\).
  \end{itemize}
  

  % ----------------------------------------------
  
  \medskip
  
  \noindent
  \textbf{Case} (\(\var := \var[w] - k\))
  % 
  Take \(\eta \in \bCnr\) and assume
  \(\max(\semnr{\var := \var[w] - k}\eta \var[y]) > \bound{\var := \var[w] - k} = k\).
  %
  Recall that
  \(\semnr{\var := \var[w] - k}\eta = \eta[\var \mapsto \eta \var[w] - k]\).
  
  We distinguish two cases:
  \begin{itemize}
    
  \item If \(\var[y] \neq \var\), then for all
    \(\eta' \in \bCnr\) such that
    \(\eta \nrsubseteq \eta'\), we have
    \(\semnr{\var := \var[w] - k}\eta' \var[y] = \eta' \var[y]\) and thus
    \begin{center}
      \(\max(\semnr{\var := \var[w] - k}\eta' \var[y]) = \max(\eta' \var[y])\).
    \end{center}
    hence the thesis holds, with
    \(h =0 \leq \bound{\var := \var[w] - k}\) and \(\var[z] = \var[y]\).
    
  \item If \(\var = \var[y]\) then for all \(\eta' \in \bCnr\) such
    that \(\eta \nrsubseteq \eta'\), we have
    \(\semnr{\var := \var[w] - k}\eta' \var[y] = \eta' \var[w] - k\) and
    thus
    \begin{center}
      \(\max(\semnr{\var := \var[w] - k}\eta' \var[y]) = \max(\eta' \var[w]) -
      k\).
    \end{center}
    Note that the assumption \(\max(\semnr{\var := \var[w] - k}\eta \var[y]) > k\) and thus
    \(\max(\semnr{\var := \var[w] - k}\eta' \var[y]) > k\) ensures that subtraction is not
    truncated on the maximum.
    
    Hence the thesis holds, with \(h = -k\), hence \(|h| = \bound{\var := \var[w] - k}\),
    and \(\var[z] = \var[w]\).
  \end{itemize}
  
  % ----------------------------------------------
  
  \medskip
  
  \noindent
  \textbf{Case} (\(\com_1 \ndet \com_2\))
  % 
  Take \(\eta \in \bCnr\) and assume
  \(\max(\semnr{\com_1 \ndet \com_2}\eta) > \bound{\com_1 \ndet \com_2} =
  \bound{\com_1} + \bound{\com_2}\).

  Recall that
  \(\semnr{\com_1 \ndet \com_2} \eta = \semnr{\com_1}\eta \sqcup \semnr{\com_2}\eta\).
  % 
  Hence, since
  \(\max(\semnr{\com_1 \ndet \com_2} \eta \var[y]) \neq \infty\), we
  have that
  \(\max(\semnr{\com_1} \eta \var[y]) \neq \infty \neq
  \max(\semnr{\com_2}\eta \var[y])\).

  Moreover
  \begin{align*}
    \max(\semnr{\com_1 \ndet \com_2}\eta \var[y])& =  \max(\semnr{\com_1}\eta \var[y] \sqcup \semnr{\com_2}\eta \var[y]) \\ 
    & = \max \{ \max(\semnr{\com_1}\eta \var[y]), \max(\semnr{\com_2}\eta \var[y])\}
  \end{align*}

  Thus
  \(\max(\semnr{\com_1 \ndet \com_2}\eta \var[y]) =
  \max(\semnr{\com_i}\eta \var[y])\) for some \(i \in \{1,2\}\). We can
  assume, without loss of generality, that the maximum is realized
  by the first component, i.e.,
  \(\max(\semnr{\com_1 \ndet \com_2}\eta \var[y]) =
  \max(\semnr{\com_1}\eta \var[y])\). Hence, by inductive hypothesis on
  \(\com_1\), we have that there exists \(h \in \mathbb{Z}\) with
  \(|h| \leq \bound{\com_1}\) and \(\var[z] \in \Var\) such that
  \(\max(\semnr{\com_1}\eta \var[y]) = \max(\eta \var[z]) + h\) and for
  all \(\eta' \in \bCnr\), \(\eta \nrsubseteq \eta'\),
  \[
  \max(\semnr{\com_1}\eta' \var[y]) \geq \max(\eta' \var[z]) + h
  \]

  Therefore 
  \[
  \max(\semnr{\com_1 \ndet \com_2}\eta \var[y])
  = \max(\semnr{\com_1}\eta \var[y]) = \max(\eta \var[z]) + h
  \]
  %
  and and for
  all \(\eta' \in \bCnr\), \(\eta \nrsubseteq \eta'\),
  \begin{align*}
    \max(\semnr{\com_1 \ndet \com_2}\eta' \var[y])
    &= \max\{ \max(\semnr{\com_1}\eta' \var[y]),  \max(\semnr{\com_2}\eta' \var[y])\}\\
    % 
    & \geq \max(\semnr{\com_1\eta'} \var[y])\\
    %
    & \geq \max(\eta' \var[z]) + h
  \end{align*}
  with \(|h| \leq \bound{\com_1} \leq \bound{\com_1 \ndet \com_2}\), as desired.


  % ----------------------------------------------
  
  \medskip
  
  \noindent
  \textbf{Case} (\(\com_1 \seq \com_2\))
  % 
  Take \(\eta \in \bCnr\) and assume
  \(\max(\semnr{\com_1 \seq \com_2}\eta) > \bound{\com_1 \seq \com_2} =
  \bound{\com_1} + \bound{\com_2}\).
  
  Recall that
  \(\semnr{\com_1 \seq \com_2} \eta = \semnr{\com_2}(\semnr{\com_1}\eta)\).
  %
  If we define
  \begin{center}
    \(\semnr{\com_1} \eta = \eta_1\)
  \end{center}
  since \(\max(\semnr{\com_2} \eta_1 \var[y]) \neq \infty\) and
  \(\max(\semnr{\com_2} \eta_1 \var[y]) > \bound{\com_1 \seq \com_2}
  \geq \bound{\com_2}\), by inductive hypothesis on \(\com_2\), there
  are \(|h_2| \leq \bound{\com_2}\) and \(\var[w] \in \Var\) such that
  \(\max(\semnr{\com_2} \eta_1 \var[y]) = \max(\eta_1 \var[w]) + h_2\)
  and for all \(\eta_1' \in \bCnr\) with
  \(\eta_1 \nrsubseteq \eta_1'\)
  \begin{equation}
    \label{eq:seq2nr}
    \max(\semnr{\com_2} \eta_1' \var[y]) \geq \max(\eta_1' \var[w]) + h_2
    \tag{\dag}
  \end{equation}
  
  Now observe that
  \(\max(\semnr{\com_1}\eta \var[w]) = \max(\eta_1 \var[w]) >
  \bound{\com_1}\). Otherwise, if it were \(\max(\eta_1 \var[w]) \leq
  \bound{\com_1}\) we would have
  \begin{center}
    \(\max(\semnr{\com_2}\eta_1 \var[y]) = \max(\eta_1 \var[w]) + h_2 \leq
    \bound{\com_1} + \bound{\com_2} = \bound{\com_1 \seq \com_2}\),
  \end{center}
  violating the hypotheses. Moreover,
  \(\max(\semnr{\com_1}\eta \var[w]) \neq \infty\), otherwise we would
  have
  \(\max(\semnr{\com_2} \eta_1 \var[y]) = \max(\eta_1 \var[w]) + h_2 =
  \infty\), contradicting the hypotheses.  Therefore we can apply the
  inductive hypothesis also to \(\com_1\) and deduce that there are
  \(|h_1| \leq \bound{\com_1}\) and \(\var[w]' \in \Var\) such that
  \(\max(\semnr{\com_1} \eta \var[w]) = \max(\eta \var[w]') + h_1\)
  and for all \(\eta' \in \bCnr\) with \(\eta \nrsubseteq \eta'\)
  \begin{equation}
    \label{eq:seq1nr}
    \max(\semnr{\com_1} \eta' \var[w]) \geq \max(\eta' \var[w]') + h_1
    \tag{\ddag}
  \end{equation}

  Now, for all \(\eta' \in \bCnr\) with \(\eta \nrsubseteq \eta'\) we have that:
  \begin{align*}
    \max(\semnr{\com_1 \seq \com_2}\eta \var[y])
    &= \max(\semnr{\com_2}(\semnr{\com_1}\eta) \var[y])\\
    %
    & = \max(\semnr{\com_2}\eta_1 \var[y])\\
    %
    & = \max(\eta_1 \var[w]) + h_2\\
    %
    & = \max(\semnr{\com_1}\eta \var[w]) + h_2\\
    %
    &= \max(\eta \var[w]')+h_1 + h_2
  \end{align*}
  %
  and
  \begin{align*}
    \max(\semnr{\com_1 \seq \com_2}\eta' \var[y]) & = & \\ 
    \max(\semnr{\com_2}(\semnr{\com_1}\eta') \var[w]) & \geq & \\ 
    \max(\semnr{\com_1}\eta' \var[w]') + h_2 & \geq & 
    \text{by \eqref{eq:seq2}, since } \eta_1 = \semnr{\com_1}\eta \nrsubseteq \semnr{\com_1}\eta' \text{ , by monotonicity} \\
    (\max(\eta' \var[y]) +h_1) + h_2 & & \text{by \eqref{eq:seq1}}\
  \end{align*}

  Thus, the thesis holds with \(h= h_1+h_2\), as
  \(|h| =|h_1 +h_2| \leq |h_1| + |h_2| \leq \bound{\com_1} +
  \bound{\com_2} = \bound{\com_1 \seq \com_2}\), as needed.



  % ----------------------------------------------------
  
  \medskip
  
  \noindent
  \textbf{Case} (\(\fix{\com}\)) 
  %
  Let \(\eta \in \bCnr\) such that
  \(\semnr{\fix{\com}} \eta \var[y] \neq \infty\). Recall that
  \(\semnr{\fix{\com}} \eta = \lfp(\lambda \mu. (\semnr{\com}
    \mu \sqcup\eta))\). Observe that the least fixpoint of
  \(\lambda \mu. (\semnr{\com}
  \mu \sqcup\eta)\) coincides with the least
  fixpoint of
  \(\lambda \mu. (\semnr{\com} \mu  \sqcup \mu) = \lambda \mu. \semnr{ \com\ndet \tru} \mu\) above \(\eta\). Hence, if
  \begin{itemize}
  \item \(\eta_0 \veq \eta\),
  \item for all \(i\in \nat\),
    \(\eta_{i+1} \veq \semnr{\com} \eta_i \sqcup \eta_i= \semnr{\com \ndet
    \tru} \eta_i \nrsupseteq \eta_i\),
  \end{itemize}
  then we define an increasing chain \(\{\eta_i\}_{i\in \nat}\subseteq \bCnr\) such that
  \[ 
  \semnr{\fix{\com}} \eta = \textstyle\bigsqcup_{i \in \nat} \eta_i.
  \]
  Since \(\semnr{\fix{\com}} \eta \var[y] \neq \infty\), we have that
  for all \(i\in \nat\), \(\eta_i \var[y] \neq \infty\). Moreover,
  \(\textstyle\bigsqcup_{i \in \nat} \eta_i\) on \(\var[y]\) is
  finitely reached in the chain \(\{\eta_i\}_{i\in \nat}\), i.e.,
  there exists \(m \in \mathbb{N}\) such that for all \(i \geq m+1\)
  \[
  \semnr{\fix{\com}} \eta \var[y] = \eta_{i} \var[y].
  \]
  %\(\eta_m \neq \eta_{m+1}\) and 

  The inductive hypothesis holds for \(\com\) and \(\tru\), hence for
  \(\com \ndet \tru\), therefore for all \(\var \in \Var\) and
  \(j \in \{0,1, \ldots, m\}\), if \(\max(\eta_{j+1} \var) >\bound{\com\ndet \tru} =\bound{\com}\) then
  there exist \(\var[z] \in \Var\) and \(h \in \mathbb{Z}\) such that \(|h| \leq \bound{\com}\) and 
  \begin{enumerate}[label=(\alph*)]
  \item \(\infty \neq \max(\eta_{j+1} \var) = \max(\eta_j \var[z]) + h\),
  \item \(\forall \eta' \nrsupseteq \eta_j.
    \max(\semnr{\com \ndet \tru}\eta'\var) \geq \max(\eta' \var[z]) + h\).
  \end{enumerate}
  To shortly denote that the two conditions (a) and (b) hold, we write
  \[
  (\var[z],j) \to_{h} (\var, j+1)
  \]
  %   when 
  %  \(j\in  \{0, \ldots, m \}\), \(\var\in \Var\) and 
  %  %\(\max(\eta_{j+1} \var) >\bound{\com}\) hold, so that the existence of
  %   \(h \in \mathbb{Z}\) and \(\var[z] \in \Var\) such that 
  %   \(\max(\eta_{j+1} \var) = \max(\eta_j \var[z]) + h\) follows.
  %   
  %  
  
  Now, assume that for some variable \(\var[y] \in \Var\)
  \[\max(\semnr{\fix{\com}} \eta \var[y]) = \max(\eta_{m+1} \var[y]) >
  \bound{\fix{\com}} = (n+1) \bound{\com}\]
  where \(n=|\mathit{vars}(\com)|\). 
  We want to show that the thesis holds, i.e., that there exist
  \(\var[z] \in \Var\) and \(h \in \mathbb{Z}\) with
  \(|h| \leq \bound{\fix{\com}}\) such that:
  \begin{equation}\label{eq:maxendmaxstartnr}
    \max(\semnr{\fix{\com}} \eta \var[y]) = \max(\eta \var[z]) + h
    \tag{i}
  \end{equation}
  and for all \(\eta' \nrsupseteq \eta\),
  \begin{equation}\label{eq:maxmiddlemaxendnr}
    \max(\semnr{\fix{\com}} \eta' \var[y]) \geq \max(\eta' \var[z]) + h
    \tag{ii}
  \end{equation}
  
  Let us consider \eqref{eq:maxendmaxstart}. We first observe that we
  can define a path
  \begin{equation}
    \label{eq:fixnr}
    \sigma \veq (\var[y]_0, 0) \to_{h_0} (\var[y]_1, 1) \to_{h_1}
    \ldots \to_{h_m} (\var[y]_{m+1}, m+1)
  \end{equation}
  such that \(\var[y]_{m+1}=\var[y]\) and for all \(j \in \{0,\ldots, m+1\}\), 
  \(\var[y]_j\in \Var\)  and
  \(\max(\eta_{j} \var[y]_{j}) > \bound{C}\).
  %, so that for \(j\neq m+1\), \(|h_j|\leq \bound{\com}\).
  In fact, if, by contradiction, this is not the case, there  would exist an index \(i \in \{0,\ldots, m\}\) (as \(\max(\eta_{m+1} \var[y]_{m+1}) > \bound{C}\) already holds)
  such that \(\max(\eta_{i} \var[y]_{i}) \leq
  \bound{C}\), while for all
  \(j \in \{i+1,\ldots, m+1\}\), \(\max(\eta_{j} \var[y]_j) > \bound{C}\).
  Thus, in such a case, 
  we consider the nonempty path:
  \[\pi \veq (\var[y]_i, i) \to_{h_i} (\var[y]_{i+1}, i+1) \to_{h_{i+1}} \ldots
  \to_{h_m} (\var[y]_{m+1}, m+1)\]
  and we have that:
  \begin{align*}
    &\Sigma_{j=i}^m h_j =\\ 
    &\Sigma_{j=i}^m \max(\eta_{j+1} \var[y]_{j+1}) - \max(\eta_j \var[y]_{j}) =\\
    &\max(\eta_{m+1} \var[y]_{m+1}) - \max(\eta_i \var[y]_{i}) =\\
    &\max(\eta_{m+1} \var[y]) - \max(\eta_i \var[y]_{i})>\\
    &  (n+1) \bound{\com} - \bound{\com} = n \bound{\com}
  \end{align*}
  with \(|h_j| \leq \bound{\com}\) for \(j \in \{i,\ldots, m\}\). Hence
  we can apply Lemma~\ref{le:cycles} to the projection \(\pi_p\) of the nodes
  of this path \(\pi\) to the variable
  component 
  to deduce that \(\pi_p\) has a subpath which is a cycle with a strictly positive weight. 
  More precisely, there
  exist \(i \leq k_1 < k_2 \leq m+1\) such that
  \(\var[y]_{k_1} = \var[y]_{k_2}\) and
  \(h = \Sigma_{j=k_1}^{k_2-1} h_j > 0\). If we denote 
  \(\var[w] = \var[y]_{k_1} = \var[y]_{k_2}\), then we
  have  that   
  \begin{align*}
    \max(\eta_{k_2} \var[w]) & =  h_{k_2-1}  + \max(\eta_{k_2-1} \var[w]) \\
                             & =  h_{k_2-1} + h_{k_2-2} + \max(\eta_{k_2-2} \var[w])  \\
                             & = \Sigma_{j=k_1}^{k_2-1} h_j + \max(\eta_{k_1} \var[w])  \\
                             & = h +  \max(\eta_{k_1} \var[w])  
  \end{align*}
  Thus,
  \[\max(\semnr{\com \ndet \tru}^{k_2-k_1} \eta_{k_1} \var[w]) = \max(\eta_{k_1}
  \var[w]) + h\] 
  Observe that for all \(\eta' \nrsupseteq \eta_{k_1}\)
  \begin{equation}\label{prop2nr}
    \max(\semnr{\com \ndet \tru}^{k_2-k_1} \eta' \var[w]) \geq \max(\eta'
    \var[w]) + h
  \end{equation}
  Property~\eqref{prop2nr} can be shown by induction on \(k_2-k_1 \geq 1\).  
  \noindent    
  Then, an inductive argument allows us to show that for all \(r \in \mathbb{N}\):
  \begin{equation}\label{noppnr}
    \max(\semnr{\com \ndet \tru}^{r(k_2-k_1)} \eta_{k_1} \var[w]) \geq \max(\eta_{k_1}
    \var[w]) + r h
  \end{equation}  
  In fact, for \(r=0\) the claim trivially holds. Assuming the validity for \(r\geq 0\) then we have that
  \begin{align*}    
    & \max(\semnr{\com \ndet \tru}^{(r+1)(k_2-k_1)} \eta_{k_1} \var[w]) =\\
    &\max(\semnr{\com \ndet \tru}^{k_2-k_1} ( \semnr{\com \ndet \tru}^{r(k_2-k_1)} \eta_{k_1}) \var[w]) \geq & \mbox{by \eqref{prop2nr} as }\eta_{k_1} \nrsubseteq \semnr{\com \ndet \tru}^{r(k_2-k_1)} \eta_{k_1}\\
    &\max(\semnr{\com \ndet \tru}^{r(k_2-k_1)} \eta_{k_1} \var[w]) + h \geq & \mbox{by inductive hypothesis}\\
    &  \max(\eta_{k_1}\var[w])  + rh + h
    \geq 
    \max(\eta_{k_1}\var[w])  + (r+1)h
  \end{align*}

  \noindent
  However, This would contradict the hypothesis
  \(\max(\semnr{\fix{\com}} \eta \var[y]) \neq \infty\). In fact the
  inequality \eqref{noppnr} would imply
  \begin{align*}
    \max(\semnr{\fix{\com}} \eta \var[w])
    & = \max\left(\bigsqcup_{i \in \mathbb{N}} \semnr{\com
      \ndet \tru}^i \eta \var[w]\right) \\ 
    & = \max\left(\bigsqcup_{i \in \mathbb{N}} \semnr{\com \ndet
      \tru}^i \eta_{k_1} \var[w]\right)\\ 
    & = \max\left(\bigsqcup_{r \in \mathbb{N}} \semnr{\com \ndet
      \tru}^{r(k_2-k_1)} \eta_{k_1} \var[w]\right)\\
    & = \infty
  \end{align*}


  Now, from \eqref{eq:fixnr} we deduce that for all
  \(\eta' \nrsupseteq \eta_{k_1}\), for \(j \in \{ k_1, \ldots, m\}\),
  if we let \(\mu_{k_1} = \eta'\) and
  \(\mu_{j+1} = \semnr{\com \ndet \tru} \mu_j\), we have that
  \(\max(\mu_{j+1} \var[y]_{j+1}) \geq \max(\mu_{j+1} \var[y]_{j}) +
  h_j\) and thus
  \begin{equation*}
    \max(\semnr{\com \ndet \tru}^{m-k_1+1} \eta' \var[y]) = \max(\mu_{m+1}
    \var[y]_{m+1}) \geq 
    \max(\var[y]_{k_1}) + \Sigma_{i=k_1}^m h_i = \max(\eta' \var[w]) + \Sigma_{i=k_1}^m h_i
  \end{equation*}
  Since \(\eta' = \semnr{\fix{\com}} \eta \nrsupseteq \eta_{k_1}\) we conclude
  \begin{align*}
    \semnr{\fix{\com}} \eta \var[y]
    & = \semnr{\com \ndet \tru}^{m-k_1+1} \semnr{\fix{\com}} \eta \var[y]\\
    & \geq \infty + \Sigma_{i=k_1}^m h_i = \infty
  \end{align*}
  contradicting the assumption.
  
  \noindent
  Therefore, the path \(\sigma\) of \eqref{eq:fixnr} must exist, and
  consequently
  \[\max(\semnr{\fix{\com}} \eta \var[y]) = \max(\eta_{m+1} \var[y]) = \max(\eta  \var[y]_0) + \Sigma_{i=0}^m h_i\]
  and
  \(\Sigma_{i=0}^m h_i \leq \bound{\fix{\com}}=(n+1)\bound{\com}\),
  otherwise we could use the same argument above for inferring the
  contradiction \(\semnr{\fix{\com}} \eta \var[y] = \infty\).

  \medskip

  Let us now show \eqref{eq:maxmiddlemaxendnr}. Given
  \(\eta' \nrsupseteq \eta\) from \eqref{eq:fixnr} we deduce that for
  all \(j \in \{ 0, \ldots, m\}\), if we let \(\mu_0 = \eta'\) and
  \(\mu_{j+1} = \semnr{\com \ndet \tru} \mu_j\), we have that
  \[
  \max(\mu_{j+1} \var[y]_{j+1}) \geq \max(\mu_{j+1} \var[y]_{j}) + h_j.
  \]
  Therefore, since \(\semnr{\fix{\com}} \eta' \nrsupseteq \mu_{m+1}\)
  (observe that the convergence of \(\semnr{\fix{\com}} \eta' \) could
  be at an index greater than \(m+1\)), we conclude that:
  \[\max(\semnr{\fix{\com}} \eta' \var[y]) \geq \max(\mu_{m+1}
  \var[y]) = \max(\mu_{m+1} \var[y]_{m+1}) \geq \max(\eta' \var[y]_0)
  + \Sigma_{i=0}^m h_i\] as desired.
\end{proof}

Lemma~\ref{le:incnr} provides an effective algorithm for computing the
interval semantics of commands. More precisely, given a command
\(\com\), the corresponding finite set of variables
\(\Var_{\com} \veq \mathit{vars}(\com)\), and an interval environment
\(\rho : \Var_{\com} \to \nrdom\), we define
\[\max(\rho) \veq \max \{ \max(\rho\var) \mid \var \in \Var_{\com}
  \}.\]
%
Then, when computing \(\semnr{\fix{\com}} \rho\) on such \(\rho\)
having a finite domain, we can restrict to a bounded interval domain
\(\bCnr_{\com,\rho} \veq (\Var_{\com} \to \nrdom[\com,\rho]) \cup
\{ \top, \bot \}\) where
\[
  \nrdom[\com,\rho] \veq \{ S\subseteq \n \mid \max(S) \leq
  \max\{\max(\rho), \left(\left| \Var_{\com}\right| + 1 \right)
  \bound{\com}\}\}.
\]

% We could also operate uniformly on all commands, defining the
% semantics for \(\com\) in a domain with intervals bounded by
% \(\max(\rho) +\bound{\com}\)

\begin{lemma}
  Let \(\com\in \imp\) be a command. Then, for all finitely supported
  \(\eta : \Var \to \nrdom\), the abstract semantics
  \(\semnr{\fix{\com}} \eta = \lfp(\lambda \mu . (\eta \sqcup
  \semnr{\com}\mu))\)
  % 
  % \semnr{\fix{\com}} \rho & = \lfp{\lambda \rho'. (\semnr{\com} \rho')
  % \sqcup \rho}
  computed in \(\bCnr\) and in \(\bCnr_{\com,\rho}\)
  coincide.
\end{lemma}

\begin{proof}
  %% Todo: consequence of Lemma~\ref{le:incnr}.
\end{proof}
